uexp/src/uexp/TDP.lean
@@ -7,45 +7,6 @@ section TDP
 
 open tactic
 
-meta def swap_ith_sigma_forward (i : nat)
-  : usr_sigma_repr → tactic unit
-| ⟨xs, body⟩ := do
-  swapped_schemas ← list.swap_ith_forward i xs,
-  -- We have to subtract because the de Bruijn indices are inside-out
-  let num_free_vars := list.length xs,
-  let swapped_body := expr.swap_free_vars (num_free_vars - 1 - i) (num_free_vars - 1 - nat.succ i) body,
-  let swapped_repr := usr_sigma_repr.mk swapped_schemas swapped_body,
-  normal_expr ← sigma_repr_to_sigma_expr ⟨xs, body⟩,
-  swapped_expr ← sigma_repr_to_sigma_expr swapped_repr,
-  equality_lemma ← to_expr ``(%%normal_expr = %%swapped_expr),
-  eq_lemma_name ← mk_fresh_name,
-  tactic.assert eq_lemma_name equality_lemma,
-  repeat_n i $ applyc `congr_arg >> funext,
-  applyc `sig_commute,
-  eq_lemma ← resolve_name eq_lemma_name >>= to_expr,
-  rewrite_target eq_lemma,
-  clear eq_lemma
-
-meta def move_once (i: nat) : tactic unit := do
-  lr ← get_lhs_sigma_repr,
-  swap_ith_sigma_forward i lr
-
-meta def move_to_front (i : nat) : tactic unit :=
-  let loop : ℕ → tactic unit → tactic unit :=
-      λ iter_num next_iter, do
-        lr ← get_lhs_sigma_repr,
-        swap_ith_sigma_forward iter_num lr,
-        next_iter
-  in nat.repeat loop i $ return ()
-
---move back i to j
-meta def move_sig_back (i: nat) (j: nat) :=
-  let loop: nat → tactic unit → tactic unit :=
-    λ num next, do 
-      next, 
-      move_once (i+num)
-  in nat.repeat loop (j-i) $ return ()
-
 meta def break_p : expr →  tactic (list expr)
 | `(%%a ≃ %%b) := 
   match a, b with
@@ -156,66 +117,9 @@ meta def normalize_sig_body : tactic unit := do
     tactic.clear eq_lemma_name
   end
 
--- a single step removal
 meta def removal_step : tactic unit := do
-  lr ← get_lhs_sigma_repr,
-  match lr with 
-  | ⟨xs, body⟩ := do 
-    le ← ra_product_to_repr body,
-    match list.head le with
-    | `(%%a ≃ %%b) := 
-      match a, b with
-      | (expr.var n), e := do 
-        let l := (list.length xs),
-        move_sig_back (l - 1 - n) (l - 1),
-        lr' ← get_lhs_sigma_repr,
-        match lr' with 
-        | ⟨xs', body'⟩ := do 
-          match body' with 
-          | `((%%c ≃ %%d) * %%f) := do
-            let sub_expr := expr.subst_var' c d f, 
-            let new_body := expr.lower_vars sub_expr 1 1,
-            old_expr ← sigma_repr_to_sigma_expr lr',
-            new_expr ←  sigma_repr_to_sigma_expr ⟨list.take (l-1) xs', new_body⟩, 
-            eq_lemma ← tactic.to_expr ``(%%old_expr = %%new_expr),
-            lemma_name ← tactic.mk_fresh_name,
-            tactic.assert lemma_name eq_lemma,
-            repeat_n (l-1) $ tactic.applyc `congr_arg >> tactic.funext,
-            tactic.applyc `sig_eq_subst_r,
-            eq_lemma_name ← tactic.resolve_name lemma_name >>= tactic.to_expr,
-            tactic.rewrite_target eq_lemma_name,
-            tactic.clear eq_lemma_name
-          | _ := tactic.fail "fail in removal step"
-          end 
-        end
-      | e, (expr.var n) := do 
-        let l := (list.length xs),
-        move_sig_back (l - 1 - n) (l - 1),
-        lr' ← get_lhs_sigma_repr,
-        match lr' with 
-        | ⟨xs', body'⟩ := do 
-          match body' with 
-          | `((%%c ≃ %%d) * %%f) := do
-            let sub_expr := expr.subst_var' d c f, 
-            let new_body := expr.lower_vars sub_expr 1 1,
-            old_expr ← sigma_repr_to_sigma_expr lr',
-            new_expr ←  sigma_repr_to_sigma_expr ⟨list.take (l-1) xs', new_body⟩, 
-            eq_lemma ← tactic.to_expr ``(%%old_expr = %%new_expr),
-            lemma_name ← tactic.mk_fresh_name,
-            tactic.assert lemma_name eq_lemma,
-            repeat_n (l-1) $ tactic.applyc `congr_arg >> tactic.funext,
-            tactic.applyc `sig_eq_subst_l,
-            eq_lemma_name ← tactic.resolve_name lemma_name >>= tactic.to_expr,
-            tactic.rewrite_target eq_lemma_name,
-            tactic.clear eq_lemma_name
-          | _ := tactic.fail "fail in removal step"
-          end 
-        end
-      | _, _ := return ()
-      end
-    | _ := return ()
-    end 
-  end
+  lhs ← get_lhs,
+  remove_sig_step lhs
 
 meta def remove_dup_sigs : tactic unit := do 
   -- this is a workround, this unnest 3 levels of pair
@@ -294,7 +198,7 @@ meta def unify_sigs : tactic unit :=
 meta def TDP' (easy_case_solver : tactic unit) : tactic unit :=
   let loop (iter_num : ℕ) (next_iter : tactic unit) : tactic unit :=
       next_iter <|> do
-      move_to_front iter_num,
+      move_sig_to_front iter_num,
       to_expr ``(congr_arg usr.sig) >>= apply,
       funext,
       easy_case_solver <|> TDP'
